add Aeneas library proxy

examples/sha3/proofs/Aeneas.lean
@@ -1,70 +1,21 @@
-import Hax
+import Aeneas.Array
+import Aeneas.Ops
+import Lean
 
 namespace Aeneas
 
-abbrev Result := RustM
-abbrev Error := _root_.Error
-abbrev ControlFlow := core_models.ops.control_flow.ControlFlow
-
-namespace Result
-
-def ok {α : Type} (v : α) : Result α := RustM.ok v
-
-end Result
-
-def lift {α : Type} (x : α) : Result α := .ok x
-
 namespace Std
 
-abbrev Usize := USize64
-abbrev U64 := UInt64
 
 scoped notation:max n "#usize" => (USize64.ofNat n)
 scoped notation:max n "#u64" => (UInt64.ofNat n)
 
-instance : HMul Usize Usize (Result Usize) where
-  hMul x y := x *? y
-
-instance : HAdd Usize Usize (Result Usize) where
-  hAdd x y := x +? y
-
-instance : HMul U64 U64 (Result U64) where
-  hMul x y := x *? y
-
-instance : HAdd U64 U64 (Result U64) where
-  hAdd x y := x +? y
 
 instance : LT Usize := inferInstanceAs (LT USize64)
 instance : DecidableLT Usize := inferInstanceAs (DecidableLT USize64)
 
 instance : HXor U64 U64 U64 := inferInstanceAs (HXor UInt64 UInt64 UInt64)
 
-abbrev Array (α : Type) (n : Usize) := RustArray α n
-abbrev Slice (α : Type) := RustSlice α
-
-def Array.index_usize {α : Type} {n : Usize} (a : Array α n) (i : Usize) : Result α :=
-  if h : i.toNat < a.toVec.size then
-    .ok (a.toVec.get ⟨i.toNat, h⟩)
-  else
-    .fail .arrayOutOfBounds
-
-def Array.update {α : Type} {n : Usize} (a : Array α n) (i : Usize) (v : α) : Result (Array α n) :=
-  if h : i.toNat < a.toVec.size then
-    .ok (.ofVec (a.toVec.set i.toNat v))
-  else
-    .fail .arrayOutOfBounds
-
-def Array.make (n : Usize) (l : List α) : Array α n :=
-  .ofVec (Vector.mk ⟨l⟩ sorry)
-
-def Array.repeat (n : Usize) (v : α) : Array α n :=
-  .ofVec (Vector.replicate n.toNat v)
-
-def Array.to_slice {α : Type} {n : Usize} (a : Array α n) : Slice α :=
-  ⟨a.toVec.toArray, by sorry⟩
-
-def Slice.len {α : Type} (s : Slice α) : Usize :=
-  USize64.ofNat s.val.size
 
 end Std
 
@@ -117,3 +68,7 @@ register_option linter.hashCommand : Bool := {
   defValue := false
   descr    := "Dummy option"
 }
+
+
+initialize do pure () <*
+  Lean.Meta.registerSimpAttr `global_simps "dummy simp-attr"
