examples/sha3/proofs/Aeneas/Array.lean
@@ -1,0 +1,33 @@
+import Aeneas.Num
+import Aeneas.Result
+
+namespace Aeneas.Std
+
+def Array (α : Type) (n : Usize) := { a : _root_.Array α // a.size = n.toNat}
+def Slice (α : Type) := _root_.Array α
+
+def Array.index_usize {α : Type} {n : Usize} (a : Array α n) (i : Usize) : Result α :=
+  if h : i.toNat < a.val.size then
+    .ok (a.val[i.toNat])
+  else
+    .fail .arrayOutOfBounds
+
+def Array.update {α : Type} {n : Usize} (a : Array α n) (i : Usize) (v : α) : Result (Array α n) :=
+  if h : i.toNat < a.val.size then
+    .ok ⟨a.val.set i.toNat v, sorry⟩
+  else
+    .fail .arrayOutOfBounds
+
+def Array.make (n : Usize) (l : List α) : Array α n :=
+  ⟨⟨l⟩, sorry⟩
+
+def Array.repeat (n : Usize) (v : α) : Array α n :=
+  ⟨Array.replicate n.toNat v, sorry⟩
+
+def Array.to_slice {α : Type} {n : Usize} (a : Array α n) : Slice α :=
+  a.val
+
+def Slice.len {α : Type} (s : Slice α) : Usize :=
+  USize64.ofNat s.size
+
+end Aeneas.Std
