examples/sha3/proofs/Aeneas/Num.lean
@@ -1,0 +1,8 @@
+import Aeneas.USize64
+
+namespace Aeneas.Std
+
+abbrev Usize := USize64
+abbrev U64 := UInt64
+
+end Aeneas.Std
