examples/sha3/proofs/Aeneas/Ops.lean
@@ -1,0 +1,91 @@
+import Aeneas.Result
+import Aeneas.USize64
+import Std.Tactic.Do
+
+namespace Aeneas
+
+theorem UInt64.toNat_add_of_lt {x y : UInt64} (h : x.toNat + y.toNat < 2 ^ 64) :
+    (x + y).toNat = x.toNat + y.toNat := BitVec.toNat_add_of_lt h
+
+theorem UInt64.toNat_mul_of_lt {x y : UInt64} (h : x.toNat * y.toNat < 2 ^ 64) :
+    (x * y).toNat = x.toNat * y.toNat := BitVec.toNat_mul_of_lt h
+
+
+/-- Addition on Rust integers. Panics on overflow. -/
+instance : HAdd UInt64 UInt64 (Result UInt64) where
+  hAdd x y :=
+    if x.toNat + y.toNat ≥ 2 ^ 64 then
+      .fail .integerOverflow
+    else pure (x + y)
+
+/-- Multiplication on Rust integers. Panics on overflow. -/
+instance : HMul UInt64 UInt64 (Result UInt64) where
+  hMul x y :=
+    if x.toNat * y.toNat ≥ 2 ^ 64 then
+      .fail .integerOverflow
+    else pure (x * y)
+
+/-- Addition on Rust integers. Panics on overflow. -/
+instance : HAdd USize64 USize64 (Result USize64) where
+  hAdd x y :=
+    if x.toNat + y.toNat ≥ 2 ^ 64 then
+      .fail .integerOverflow
+    else pure (x + y)
+
+/-- Multiplication on Rust integers. Panics on overflow. -/
+instance : HMul USize64 USize64 (Result USize64) where
+  hMul x y :=
+    if x.toNat * y.toNat ≥ 2 ^ 64 then
+      .fail .integerOverflow
+    else pure (x * y)
+
+open Std.Do
+set_option mvcgen.warning false
+
+@[spec]
+theorem USize64.mul_spec (x y : USize64)
+    (h1 : x.toNat * y.toNat ≥ 2 ^ 64 → (Q.2.1 Error.integerOverflow).down)
+    (h2 : ∀ r : USize64, r.toNat = x.toNat * y.toNat → (Q.1 r).down) :
+    ⦃ ⌜ True ⌝ ⦄
+    (x * y)
+    ⦃ Q ⦄ := by
+  unfold HMul.hMul; dsimp [instHMulUSize64Result]
+  mvcgen
+  · apply h1 (by assumption)
+  · apply h2; rw [USize64.toNat_mul_of_lt]; grind
+@[spec]
+
+theorem UInt64.mul_spec (x y : UInt64)
+    (h1 : x.toNat * y.toNat ≥ 2 ^ 64 → (Q.2.1 Error.integerOverflow).down)
+    (h2 : ∀ r : UInt64, r.toNat = x.toNat * y.toNat → (Q.1 r).down) :
+    ⦃ ⌜ True ⌝ ⦄
+    (x * y)
+    ⦃ Q ⦄ := by
+  unfold HMul.hMul; dsimp [instHMulUInt64Result]
+  mvcgen
+  · apply h1 (by assumption)
+  · apply h2; rw [UInt64.toNat_mul_of_lt]; grind
+
+@[spec]
+theorem USize64.add_spec (x y : USize64)
+    (h1 : x.toNat + y.toNat ≥ 2 ^ 64 → (Q.2.1 Error.integerOverflow).down)
+    (h2 : ∀ r : USize64, r.toNat = x.toNat + y.toNat → (Q.1 r).down) :
+    ⦃ ⌜ True ⌝ ⦄
+    (x + y)
+    ⦃ Q ⦄ := by
+  unfold HAdd.hAdd; dsimp [instHAddUSize64Result]
+  mvcgen
+  · apply h1 (by assumption)
+  · apply h2; rw [USize64.toNat_add_of_lt]; grind
+@[spec]
+
+theorem UInt64.add_spec (x y : UInt64)
+    (h1 : x.toNat + y.toNat ≥ 2 ^ 64 → (Q.2.1 Error.integerOverflow).down)
+    (h2 : ∀ r : UInt64, r.toNat = x.toNat + y.toNat → (Q.1 r).down) :
+    ⦃ ⌜ True ⌝ ⦄
+    (x + y)
+    ⦃ Q ⦄ := by
+  unfold HAdd.hAdd; dsimp [instHAddUInt64Result]
+  mvcgen
+  · apply h1 (by assumption)
+  · apply h2; rw [UInt64.toNat_add_of_lt]; grind
