examples/sha3/proofs/Aeneas/Result.lean
@@ -1,0 +1,84 @@
+import Std
+
+namespace Aeneas
+/--
+  (Aeneas) Error cases
+-/
+inductive Error where
+   | assertionFailure: Error
+   | integerOverflow: Error
+   | divisionByZero: Error
+   | arrayOutOfBounds: Error
+   | maximumSizeExceeded: Error
+   | panic: Error
+   | undef: Error
+deriving Repr, BEq, DecidableEq
+open Error
+
+/--
+  RustM monad (corresponding to Aeneas's `Result` monad), representing
+  possible results of rust computations.
+
+  Defined as `ExceptT Error Option`, i.e. `Option (Except Error α)`.
+  The `Option` layer models divergence and the `Except Error` layer models
+  Rust panics. The `ExceptT` transformer ensures that once a program has
+  paniced, it can not diverge any more (and vice versa).
+-/
+def Result (α : Type) := ExceptT Error Option α
+
+namespace Result
+
+-- These `Except` instances are missing in Lean's library.
+-- We use them to derive the corresponding `Result` instances below.
+deriving instance BEq, DecidableEq for Except
+
+instance instBEq {α : Type} [BEq α] : BEq (Result α) :=
+  inferInstanceAs (BEq (Option (Except Error α)))
+instance instDecidableEq {α : Type} [DecidableEq α] : DecidableEq (Result α) :=
+  inferInstanceAs (DecidableEq (Option (Except Error α)))
+instance instInhabited {α : Type} : Inhabited (Result α) :=
+  inferInstanceAs (Inhabited (Option (Except Error α)))
+instance instMonad : Monad Result :=
+  inferInstanceAs (Monad (ExceptT Error Option))
+instance instLawfulMonad : LawfulMonad Result :=
+  inferInstanceAs (LawfulMonad (ExceptT Error Option))
+
+@[reducible, match_pattern] def ok {α : Type} (v : α) : Result α := some (.ok v)
+@[reducible, match_pattern] def fail {α : Type} (e : Error) : Result α := some (.error e)
+@[reducible, match_pattern] def div {α : Type} : Result α := none
+
+instance {α : Type} [Repr α] : Repr (Result α) where
+  reprPrec x prec := match x with
+    | .ok v   => Repr.addAppParen (f!"Result.ok {reprArg v}") prec
+    | .fail e => Repr.addAppParen (f!"Result.fail {reprArg e}") prec
+    | .div    => "Result.div"
+
+def ofOption {α : Type} (x : Option α) (e : Error) : Result α :=
+  match x with
+  | .some v => pure v
+  | .none => .fail e
+
+@[reducible]
+def isOk {α : Type} (x : Result α) : Bool :=
+  match x with
+  | .ok _ => true
+  | _ => false
+
+@[reducible]
+def of_isOk {α : Type} (x : Result α) (h : Result.isOk x) : α :=
+  match x with
+  | .ok v => v
+
+@[simp, spec]
+def ok_of_isOk {α : Type} (v : α) (h : isOk (ok v)) : (ok v).of_isOk h = v := by rfl
+
+open Std.Do
+
+instance instWP : WP Result (.except Error (.except PUnit .pure)) :=
+  inferInstanceAs (WP (ExceptT Error Option) _)
+instance instWPMonad : WPMonad Result (.except Error (.except PUnit .pure)) :=
+  inferInstanceAs (WPMonad (ExceptT Error Option) _)
+
+abbrev holds (x : Result Prop) : Prop := ⦃ ⌜ True ⌝ ⦄ x ⦃ ⇓ p => ⌜ p ⌝ ⦄
+
+def lift {α : Type} (x : α) : Result α := .ok x
