examples/sha3/proofs/Sha3/Equivalence.lean
@@ -1,0 +1,14 @@
+import Sha3.Funs
+
+namespace sha3
+
+-- The reference implementation
+#check reference.iota
+
+-- The real implementaion
+#check KeccakState.iota
+
+theorem KeccakState.iota_spec :
+  ⦃ ⌜ True ⌝ ⦄
+  KeccakState.iota
+  ⦃ ⇓ r => ⌜ ⌝ ⦄
